src/rocq/Semantics/Compare.v
@@ -1,0 +1,43 @@
+From Vellvm Require Import
+  Utilities
+  Syntax
+  Numeric.Rocqlib
+  Numeric.Integers
+  Numeric.Floats
+  Semantics.DynamicValues
+  Semantics.MemoryParams
+  Semantics.LLVMParams.
+
+From ExtLib Require Import
+     Structures.Monads.
+ 
+Module COMPARE (LP : LLVMParams) (MP : MEMORY_PARAMS LP).
+  Import MP.
+  Import LP.
+  Import SZ.
+  Import DV.
+  Import MBYTES.
+  Import PTOI.
+  
+  Definition eval_icmp {M} `{Monad M} `{RAISE_ERROR M} (samesign:bool) (icmp : icmp) (v1 v2 : dvalue) : M dvalue.
+    refine
+      (match v1, v2 with
+       | @DVALUE_I sz1 i1, @DVALUE_I sz2 i2 =>
+           _
+       | DVALUE_IPTR i1, DVALUE_IPTR i2 => eval_int_icmp samesign icmp i1 i2
+       | DVALUE_Poison t1, DVALUE_Poison t2 => ret (DVALUE_Poison t1)
+       | DVALUE_Poison t, _ => if is_DVALUE_IX v2 then ret (DVALUE_Poison t) else raise_error "ill_typed-iop"
+       | _, DVALUE_Poison t => if is_DVALUE_IX v1 then ret (DVALUE_Poison t) else raise_error "ill_typed-iop"
+       | DVALUE_Addr a1, DVALUE_Addr a2 =>
+           let i1 := ptr_to_int a1 in
+           let i2 := ptr_to_int a2 in
+           eval_int_icmp false icmp i1 i2
+       | _, _ => raise_error ("ill_typed-icmp: " ++ show_dvalue v1 ++ ", " ++ show_dvalue v2)
+       end).
+    destruct (Pos.eq_dec sz1 sz2); subst.
+    - exact (eval_int_icmp samesign icmp i1 i2).
+    - exact (raise_error ("ill_typed-icmp: " ++ show_dvalue v1 ++ ", " ++ show_dvalue v2)).
+  Defined.
+  Arguments eval_icmp _ _ _ _ : simpl nomatch.
+
+End COMPARE.
