src/rocq/Semantics/GepM.v
@@ -1,20 +1,10 @@
-From Stdlib Require Import ZArith String List Lia.
-
-From ExtLib Require Import
-     Structures.Monad
-     Structures.Functor.
-
 From Vellvm Require Import
-  DynamicTypes
+  Utilities
+  Syntax
   VellvmIntegers
   Semantics.LLVMParams
   Semantics.MemoryAddress
-  Semantics.Memory.Sizeof
-  Utils.Error
-  Utils.Tactics.
-
-Import ListNotations.
-Import MonadNotation.
+  Semantics.Memory.Sizeof.
 
 Module Type GEPM (LP:LLVMParams).
   Import LP.DV.
@@ -34,7 +24,7 @@ Module Type GEPM (LP:LLVMParams).
       The offset is therefore incremented by this index times the size of the type of elements stored. Finally, a recursive call
       at this new offset allows for deeper unbundling of a nested structure.
    *)
-  Fixpoint handle_gep_h (t:dtyp) (off:Z) (vs:list dvalue): err Z :=
+  Fixpoint handle_gep_h (t:dtyp) (off:Z) (vs:list dvalue): EOB Z :=
     match vs with
     | v :: vs' =>
       match v with
@@ -45,7 +35,7 @@ Module Type GEPM (LP:LLVMParams).
         | DTYPE_Array _ ta
         | DTYPE_Vector _ ta =>
             handle_gep_h ta (off + k * (Z.of_N (sizeof_dtyp ta))) vs'
-        | _ => failwith ("non-i8-indexable type")
+        | _ => raise_error ("non-i8-indexable type")
         end
       | @DVALUE_I 32 i =>
         let k := unsigned i in
@@ -59,7 +49,7 @@ Module Type GEPM (LP:LLVMParams).
             let offset := fold_left (fun acc t => pad_to_align (dtyp_alignment t) acc + sizeof_dtyp t)%N
                             (firstn n ts) 0%N in
             match nth_error ts n with
-            | None => failwith "overflow"
+            | None => raise_error "overflow"
             | Some t' =>
                 handle_gep_h t' (off + Z.of_N offset) vs'
             end
@@ -67,11 +57,11 @@ Module Type GEPM (LP:LLVMParams).
           let offset := fold_left (fun acc t => acc + sizeof_dtyp t)%N
                                   (firstn n ts) 0%N in
           match nth_error ts n with
-          | None => failwith "overflow"
+          | None => raise_error "overflow"
           | Some t' =>
             handle_gep_h t' (off + Z.of_N offset) vs'
           end
-        | _ => failwith ("non-i32-indexable type")
+        | _ => raise_error ("non-i32-indexable type")
         end
       | @DVALUE_I 64 i =>
         let k := signed i in
@@ -80,7 +70,7 @@ Module Type GEPM (LP:LLVMParams).
         | DTYPE_Array _ ta
         | DTYPE_Vector _ ta =>
             handle_gep_h ta (off + k * (Z.of_N (sizeof_dtyp ta))) vs'
-        | _ => failwith ("non-i64-indexable type")
+        | _ => raise_error ("non-i64-indexable type")
         end
       | DVALUE_IPTR i =>
         let k := to_Z i in
@@ -89,9 +79,9 @@ Module Type GEPM (LP:LLVMParams).
         | DTYPE_Array _ ta
         | DTYPE_Vector _ ta =>
             handle_gep_h ta (off + k * (Z.of_N (sizeof_dtyp ta))) vs'
-        | _ => failwith ("non-iptr-indexable type")
+        | _ => raise_error ("non-iptr-indexable type")
         end
-      | _ => failwith "handle_gep_h: unsupported index type"
+      | _ => raise_error "handle_gep_h: unsupported index type"
       end
     | [] => ret off
     end.
@@ -100,7 +90,7 @@ Module Type GEPM (LP:LLVMParams).
      The pointer set the block into which we look, and the initial offset. The first index value add to the initial offset passed to [handle_gep_h] for the actual access to structured data.
    *)
   (* TODO: This should take into account padding too... May break get_consecutive_ptrs and friends. *)
-  Definition handle_gep_addr (t:dtyp) (a:addr) (vs:list dvalue) : err (OOM addr) :=
+  Definition handle_gep_addr {M} `{Monad M} `{RAISE_ERROR M} `{RAISE_OOM M} (t:dtyp) (a:addr) (vs:list dvalue) : M addr :=
     let ptr := ptr_to_int a in
     let prov := address_provenance a in
     match vs with
@@ -185,106 +175,6 @@ Module Type GEPM (LP:LLVMParams).
     inv IX.
     auto.
   Qed.
-
-  (* Lemma handle_gep_addr_cons_inv : *)
-  (*   forall t base_addr idx idxs final_addr, *)
-  (*     handle_gep_addr t base_addr (idx :: idxs) = inr (ret final_addr) -> *)
-  (*     exists res_addr, *)
-  (*       handle_gep_addr t base_addr [idx] = inr (ret res_addr) /\ *)
-  (*         handle_gep_addr t res_addr idxs = inr (ret res_addr). *)
-  (* Proof. *)
-  (*   intros t base_addr idx idxs final_addr H. *)
-  (*   cbn in H. *)
-  (*   break_match_hyp_inv. *)
-  (*   - break_match_hyp_inv. *)
-  (*     exists final_addr. *)
-
-
-  (*     remember (int_to_ptr (ptr_to_int base_addr + Z.of_N (sizeof_dtyp t) * DynamicValues.Int8.unsigned x) (address_provenance base_addr)). *)
-  (*     pose proof int_to_ptr_ptr_to_int_exists. *)
-  (*     exists (int_to_ptr (ptr_to_int base_addr + Z.of_N (sizeof_dtyp t) * DynamicValues.Int8.unsigned x) (address_provenance base_addr)). *)
-
-  (* Qed. *)
-
-  (* Lemma handle_gep_h_cons : *)
-  (*   forall idxs idx t base_addr res_addr final_addr, *)
-  (*     handle_gep_h t base_addr [idx] = inr res_addr -> *)
-  (*     handle_gep_h t res_addr idxs = inr final_addr -> *)
-  (*     handle_gep_h t base_addr (idx :: idxs) = inr final_addr. *)
-  (* Proof. *)
-  (*   intros idxs. *)
-  (*   induction idxs; intros idx t base_addr res_addr final_addr GEP_START GEP_REST. *)
-  (*   - cbn in GEP_REST. inv GEP_REST; auto. *)
-  (*   - specialize  *)
-  (*     cbn in GEP_REST. *)
-  (*     break_match_hyp_inv. *)
-  (*     + break_match_hyp_inv. *)
-  (*       specialize x (res_addr + DynamicValues.Int8.unsigned x * Z.of_N (sizeof_dtyp d)) *)
-  (*       * cbn in H1. *)
-
-  (*     specialize (IHidxs a t res_addr). *)
-      
-      
-  (*   cbn; cbn in GEP_START. *)
-  (*   break_match_hyp_inv. *)
-  (*   - break_match_hyp_inv. *)
-  (*     + generalize dependent final_addr. *)
-  (*       generalize dependent base_addr. *)
-  (*       induction idxs; intros base_addr final_addr GEP_REST. *)
-  (*       * cbn in *; auto. *)
-  (*       * cbn in *. *)
-  (*         break_match_hyp_inv. *)
-  (*         --  *)
-  (* Qed. *)
-
-  (* Lemma handle_gep_addr_cons : *)
-  (*   forall idx idxs t base_addr res_addr final_addr, *)
-  (*     handle_gep_addr t base_addr [idx] = inr (ret res_addr) -> *)
-  (*     handle_gep_addr t res_addr idxs = inr (ret final_addr) -> *)
-  (*     handle_gep_addr t base_addr (idx :: idxs) = inr (ret final_addr). *)
-  (* Proof. *)
-  (*   intros idx. *)
-  (*   induction idxs; intros t base_addr res_addr final_addr GEP_START GEP_REST. *)
-  (*   - cbn in GEP_REST. inv GEP_REST. *)
-  (*   - cbn in GEP_START. *)
-  (*     cbn. *)
-  (*     break_match_hyp_inv. *)
-  (*     + cbn in GEP_REST. *)
-  (*       break_match_hyp_inv. *)
-  (*       * break_match_hyp_inv. *)
-  (*         break_match_goal. *)
-  (*         admit. *)
-
-  (*         break_match_hyp_inv. *)
-          
-      
-
-  (*   intros t base_addr idx idxs res_addr final_addr GEP_START GEP_REST. *)
-  (*   cbn. *)
-  (*   cbn in GEP_START. *)
-  (*   break_match_hyp_inv. *)
-  (*   - unfold handle_gep_addr in GEP_REST. *)
-  (*     induction idxs; inv GEP_REST. *)
-  (*     forward IHidxs. *)
-      
-      
-  (*     generalize dependent res_addr. *)
-  (*     induction idxs; intros res_addr GEP_REST H0. *)
-  (*     + inv GEP_REST. *)
-  (*     + cbn. *)
-  (*       setoid_rewrite GEP_REST. *)
-  (*     break_match_goal. *)
-  (*     + unfold handle_gep_addr in GEP_REST. *)
-  (*       break_match_hyp_inv. *)
-  (*       break_match_hyp_inv. *)
-  (*       cbn in *. *)
-  (*       break_match_hyp_inv. *)
-  (*       break_match_hyp_inv. *)
-
-                             
-        
-  (*   reflexivity. *)
-  (* Qed. *)
 
   Lemma handle_gep_addr_preserves_provenance :
     forall (dt : dtyp) ixs (p p' : addr),
