src/rocq/Utils/EOB.v
@@ -1,0 +1,59 @@
+From Stdlib Require Import
+  String List.
+From ExtLib Require Import
+  Structures.Monads.
+From Vellvm.Utils Require Import
+  ListUtil Tactics.
+
+Definition empty_elim (X : Type) : Empty_set -> X :=
+  fun abs => match abs with end.
+
+Variant EOB {X : Type} : Type :=
+  | raise_oom (s : string) : EOB
+  | raise_ub (s : string) : EOB
+  | raise_error (s : string): EOB
+  | raise_ret (x : X) : EOB.
+Arguments EOB: clear implicits.
+
+#[global] Instance EOB_monad : Monad EOB :=
+  {| ret := @raise_ret ;
+    bind _ _ c k :=
+      match c with
+      | raise_oom s => raise_oom s
+      | raise_ub  s => raise_ub s
+      | raise_error s => raise_error s
+      | raise_ret x => k x
+      end
+  |}.
+
+Lemma map_monad_EOB_Forall2 :
+  forall {A B} (f : A -> EOB B) l res,
+    map_monad f l = ret res <->
+      Forall2 (fun a b => f a = ret b) l res.
+Proof.
+  induction l as [| a l IH]; cbn; intros ?.
+  - split.
+    + intros EQ; inv EQ; auto.
+    + intros F; inv F; auto.
+  - split.
+    + intros EQ; break_match_hyp; abs_eq.
+      break_match_hyp; abs_eq.
+      inv EQ.
+      apply Forall2_cons; auto.
+      now apply IH.
+    + intros HF; inv HF.
+      rw_match.
+      apply IH in H3.
+      rw_match; auto.
+Qed.
+
+Lemma map_monad_EOB_success A B (f : A -> EOB B) (l : list A) b :
+  map_monad f l = ret b ->
+  forall a, In a l -> exists b, f a = ret b.
+Proof.
+  intros EQ; apply map_monad_EOB_Forall2 in EQ.
+  induction EQ.
+  - cbn; easy.
+  - intros ? [<- | IN]; eauto.
+Qed.
+
