src/rocq/Utils/OptionUtil.v
@@ -1,32 +1,6 @@
-From ExtLib Require Import
-  Structures.Foldable.
-
-Definition guard_opt (x : bool) : option unit
-  := if x then Some tt else None.
-
 Definition from_option {A} (def : A) (opt : option A) : A
   := match opt with
      | Some x => x
      | None => def
      end.
 
-Definition option_rel2 {X1 X2 : Type} (R : X1 -> X2 -> Prop) : (option X1 -> option X2 -> Prop) :=
-  fun mx my => match mx,my with
-            | Some x, Some y => R x y
-            | None, None => True
-            | _, _ => False
-            end.
-#[export] Hint Unfold option_rel2 : core.
-
-Import Monoid.
-#[global] Instance Foldable_option {a} : Foldable (option a) a.
-split.
-intros m M conv oa.
-apply (match oa with | Some a => conv a | None => (monoid_unit M) end).
-Defined.
-
-Definition maybe {a b} (def : b) (f : a -> b) (oa : option a) : b
-  := match oa with
-     | Some a => f a
-     | None => def
-     end.
