src/rocq/Utils/StringUtil.v
@@ -1,0 +1,20 @@
+From Stdlib Require Import String Ascii List.
+From Vellvm.Utils Require Import ListUtil.
+Import ListNotations.
+
+Fixpoint string_fold_left {A} (f : A -> ascii -> A) (s:string) (acc:A) : A :=
+  match s with
+  | EmptyString => acc
+  | String ch s =>
+      string_fold_left f s (f acc ch)
+  end.
+
+Definition rev_string (s : string) : string
+  := string_fold_left (fun acc x => String x acc) s EmptyString.
+
+Definition string_of_list_ascii_tail_rec (s : list ascii) : string
+  := rev_string (fold_left (fun acc ch => String ch acc) s EmptyString).
+
+Definition list_ascii_of_string_tail_rec (s : string) : list ascii
+  := rev_tail_rec (string_fold_left (fun acc ch => ch :: acc) s []).
+
