src/rocq/Utils/BoolUtil.v
@@ -1,0 +1,6 @@
+Definition option_pred {A} (pred : A -> bool) (ma : option A) : bool
+  := match ma with
+     | Some x => pred x
+     | None => false
+     end.
+
